src/contracts_coq/contract_components.v
@@ -1,0 +1,14 @@
+Require Import String ZArith.
+Require Import syntax macros semantics comparable util.
+Import error.
+Require tez.
+Require map.
+
+
+Module Contract_components (C : ContractContext).
+
+Module semantics := Semantics C. Import semantics.
+
+
+
+End Contract_components.
