src/contracts_coq/spending_limit_contract_definition.v
@@ -1,0 +1,375 @@
+
+Require Import Michocoq.macros.
+Import syntax.
+Import comparable.
+Require Import ZArith.
+Require Import String.
+Require Import semantics.
+Require Import util.
+Import error.
+Require List.
+
+Require Import typer.
+Require tez.
+Require map.
+
+Import List.ListNotations.
+
+Definition payload_ty :=
+  or
+    (pair
+       (pair
+          (* %journaliere) *)
+          key_hash
+          (pair
+             (pair
+                (*
+                 * %fonds_restant
+                 *)
+                mutez
+                (*
+                 * %duree_de_blocage
+                 *)
+                int)
+             (* %file *)
+             (pair
+                (list (pair timestamp mutez))
+                (list (pair timestamp mutez)))))
+       (*  %nouvelle_clef_maitresse *)
+       key_hash)
+    None
+    (pair
+       (lambda unit (list operation))
+       (*  %nouvelle_clef_publique *)
+       key_hash)
+    None.
+
+Definition parameter_master_ty :=
+  (pair
+     (pair
+        (* %clef_publique) *)
+        key signature)
+     payload_ty).
+
+Definition parameter_transfer_ty :=
+  (pair (*  %transfer *)
+     (pair
+        (list (*  %beneficiaires *)
+           (pair
+              (* %montant *)
+              mutez
+              (*  %beneficiaire *)
+              (contract unit)))
+        (* %novelle_clef_journaliere *)
+        key_hash)
+     (pair
+        (* %clef_publique *)
+        key
+        signature)).
+
+Definition parameter_ty : type :=
+  (or
+      (*
+       * %send
+       *)
+     unit
+     (Some "%send"%string)
+     (or
+        parameter_master_ty (Some "%appel_clef_maitresse"%string)
+        parameter_transfer_ty (Some "%transfer"%string)) None).
+
+Definition storage_context_ty :=
+  (pair
+     (* journaliere *)
+     key_hash
+     (pair
+        (pair
+           (*
+            * %fonds_restant
+            *)
+           mutez
+           (* %duree_de_blocage *)
+           int)
+        (* %file *)
+        (pair
+           (list (pair timestamp mutez))
+           (list (pair timestamp mutez))))).
+
+Definition storage_auth_ty :=
+  (pair
+     (* %maitresse *)
+     key_hash
+     (* %sel *)
+     (pair nat nat)).
+
+Definition storage_ty := (pair storage_context_ty storage_auth_ty).
+
+Module Spending_limit_contract_definition(C:ContractContext).
+
+Module semantics := Semantics C. Import semantics.
+
+Definition slc_ep_master_lambda :
+  instruction_seq (Some (parameter_ty, None))
+                  false
+                  ((pair
+                      (lambda unit (list operation))
+                      (*  %nouvelle_clef_publique *)
+                      key_hash) ::: (pair nat nat)::: storage_context_ty ::: nil)
+                  (list operation ::: storage_context_ty ::: storage_auth_ty ::: nil)
+  :=
+    (* execute lambda *)
+    { UNPAIR (* @function *) (* @new_master_key *) ;
+      DIP1 { PAIR; SWAP };
+      UNIT ;
+      EXEC }%michelson.
+
+Definition slc_ep_master :
+  instruction_seq (Some (parameter_ty, None))
+                  false
+                  (parameter_master_ty ::: storage_context_ty ::: storage_auth_ty ::: nil)
+                  (list operation ::: storage_context_ty ::: storage_auth_ty ::: nil) :=
+  { (* retrieve master_key and salt from storage *)
+    DIP1 {SWAP};
+    SWAP ;
+    UNPAIR ;
+    (* pack the payload with the header (contract, chain_id, salt) *)
+    DIP1 {SWAP;
+          UNPAIR;
+          DIP1 { DUP;
+                 (* pack the received payload (new storage or lambda) *)
+                 PACK (* @packedpayload *) ;
+                 (* pack the header *)
+                 DIP1 { DIP1 { UNPAIR;
+                               DUP ;
+                               DIP1 {
+                                   PUSH nat (Nat_constant 2) ;
+                                   (* increment salt *)
+                                   ADD (s := add_nat_nat) (* @salt_inc *) ;
+                                   PAIR };
+                               PACK (* @packed_salt *) ;
+                               (* packed(salt) *)
+                               CHAIN_ID ;
+                               SELF (self_type := parameter_ty) (self_annot := None) None I ;
+                               PAIR ;
+                               PACK (* @packed_self_chain_id *) ;
+                               (* packed(self, chain_id) : packed(salt) : ... *)
+                               CONCAT (i := stringlike_bytes) (* @packedheader *)
+                                      (* (packed(self, chain_id) ++ packed(salt)) : ... *)
+                             } ;
+                        SWAP} ;
+                 CONCAT (i := stringlike_bytes) (* @packedpayload *) ;
+                 (* (packed(storage) *)
+                 (*    ++ packed(self, chain_id) *)
+                 (*    ++ packed(salt)) : ... *)
+                 DUP (* @packedpayloadDup *) } ;
+          UNPAIR ;
+          DUP ;
+          HASH_KEY (* @sender_public_key_hash *)
+         } ;
+
+    (* verify that the public key hash of the sender equal the public key has of the master *)
+    ASSERT_CMPEQ ;
+    (* verify that the that the signature is a signature of the payload with from master *)
+    CHECK_SIGNATURE ;
+    (* if not, fail. *)
+    IF_TRUE {DROP1} {FAILWITH} ;
+
+    IF_LEFT { (* set new storage *)
+        UNPAIR (* @new_storage *) (* @new_master_key *) ;
+        (* pair up the incremented salt with the new master key *)
+        DIP1{ PAIR ;
+                SWAP ;
+                DROP1} ;
+        (* no operations will be executed *)
+        NIL operation}
+            ((* execute lambda *)
+              slc_ep_master_lambda
+  )}%michelson.
+
+
+Definition slc_ep_transfer2_transaction_iter_body {A}:
+  instruction_seq (Some (parameter_ty, None)) false
+              (pair mutez (contract unit) ::: list operation ::: mutez ::: A)
+              (list operation ::: mutez ::: A) :=
+  { UNPAIR ; (* production des transactions *)
+    DUP ;
+    DIP1 {
+        UNIT ;
+        TRANSFER_TOKENS ;
+        CONS
+      } ;
+    SWAP ;
+    (* #calcul du temps de blocage *)
+    DIP1 { SWAP ; ADD (s := add_tez_tez) }}%michelson.
+
+
+Definition slc_ep_transfer2_transaction_iter {A} :
+  instruction
+    (Some (parameter_ty, None))
+    false
+    (list (pair mutez (contract unit)) ::: list operation ::: mutez ::: A)
+    _
+  :=
+  ITER (i := iter_list _) (slc_ep_transfer2_transaction_iter_body).
+
+
+Definition slc_ep_transfer_loop_body :
+  instruction (Some (parameter_ty, None)) _
+  (list (pair timestamp mutez) ::: list (pair timestamp mutez) ::: mutez ::: storage_auth_ty ::: nil)
+  (bool ::: list (pair timestamp mutez) ::: list (pair timestamp mutez) ::: mutez ::: storage_auth_ty::: nil)
+  := (IF_CONS { DUP ;
+                CAR ;
+                NOW ;
+                IFCMPGE { CDR ;
+                          SWAP ;
+                          DIP1 { SWAP ;
+                                 DIP1 { ADD (s := add_tez_tez)}} ;
+                          PUSH bool True_ }
+                        { CONS ;
+                          PUSH bool False_}}
+              { IF_CONS { NIL (pair timestamp mutez) ;
+                          SWAP ;
+                          CONS ;
+                          SWAP ;
+                          ITER (i := iter_list _) { CONS } ;
+                          NIL (pair timestamp mutez) ;
+                          SWAP ;
+                          PUSH bool True_}
+                        { NIL (pair timestamp mutez) ;
+                          DUP ;
+                          PUSH bool False_}
+     })%michelson.
+
+Definition slc_ep_transfer_loop : instruction _ _ _ _ :=
+  (LOOP { slc_ep_transfer_loop_body })%michelson.
+
+Definition slc_ep_transfer1_check_signature :
+  instruction_seq (Some (parameter_ty, None)) Datatypes.false
+                  (parameter_transfer_ty ::: storage_context_ty ::: storage_auth_ty ::: nil)
+                  (list (pair mutez (contract unit)) :::
+                        list operation ::: mutez ::: key_hash ::: int ::: mutez ::: list (pair timestamp mutez) :::
+                        list (pair timestamp mutez) ::: storage_auth_ty ::: nil)
+  (*
+   * (list operation ::: mutez ::: key_hash ::: int ::: mutez :::
+   *       (list (pair timestamp mutez)) :::
+   *       (list (pair timestamp mutez)) :::
+   *       (pair key_hash nat) ::: nil)
+   *)
+  :=
+    {
+      DIP1 { UNPAPAIR } ; (* cas d'un appel simple *)
+      UNPAIR ;
+      DUP ;
+      PACK ;
+      DIP1 {
+          UNPAIR (a := list (pair mutez (contract unit)))
+                 (b := key_hash) ;
+          DIP1 {SWAP}} ;
+      SWAP ;
+      DIP1 { DIP1 { DIP1 {SWAP} ;
+                    SWAP ;
+                    DIP1 { UNPAIR ;
+                            DUP ;
+                            HASH_KEY } ;
+                    ASSERT_CMPEQ ; (* verification de compatibilite des clefs *)
+                    DIG 5 (S1 := (_ ::: _ ::: _ ::: _ ::: _ ::: nil)) (@eq_refl _ 5) ;
+                    UNPAIR ;
+                    DIP1 { UNPAIR;
+                           DIP1 { DUP ;
+                                  PUSH nat (Nat_constant 2) ;
+                                  ADD (s:= add_nat_nat) } ;
+                           PAIR };
+                    PAIR ;
+                    DUG 6 (S1 := (_ ::: _ ::: _ ::: _ ::: _ ::: _ ::: nil)) (@eq_refl _ 6) ;
+                    PACK ;
+                    CHAIN_ID ;
+                    SELF (self_type := parameter_ty) (self_annot := None) None I ;
+                    PAIR ;
+                    PACK ;
+                    CONCAT (i := stringlike_bytes)
+                } ;
+              CONCAT (i := stringlike_bytes) ;
+              SWAP ;
+              DIP1 { SWAP ;
+                      DIP1 {DUP}} ;
+              CHECK_SIGNATURE ; (* #verification de signature *)
+              IF_TRUE {DROP1} {FAILWITH} ;
+              DIP1 { UNPAIR (b := int) ;
+                     SWAP ;
+                     DIP1 { SWAP ;
+                            UNPAIR ;
+                            PUSH bool True_ ;
+                            (* recherche de fonds à liberer *)
+                            slc_ep_transfer_loop ;
+                            DIP1 {SWAP} ;
+                            SWAP
+                          }
+                  } ;
+              PUSH mutez (0 ~mutez) ;
+              NIL operation
+    }}%michelson.
+
+Definition slc_ep_transfer3_register :
+  instruction (Some (parameter_ty, None)) false
+              (list operation ::: mutez ::: key_hash ::: int ::: mutez :::
+                    list (pair timestamp mutez) :::
+                    list (pair timestamp mutez) :::
+                    storage_auth_ty ::: nil)
+              (list operation ::: storage_context_ty ::: storage_auth_ty ::: nil)
+  :=
+    DIP1 { SWAP ; (* blocage des fonds depensés *)
+           DIP1 { SWAP ;
+                  DUP ;
+                  NOW ;
+                  ADD (s := add_timestamp_int);
+                  SWAP ;
+                  DIP1 { DIP1 { SWAP } ;
+                         SWAP ;
+                         DIP1 { SWAP ;
+                                DUP ;
+                                DIP1 { SWAP ;
+                                       PAIR ;
+                                       SWAP ;
+                                       DIP1 { CONS } ; (* ajout dans la file *)
+                                       PAIR}} ;
+                         SUB (s := sub_tez_tez)} ; (* calcul du reste non bloqué *)
+                  SWAP ;
+                  PAIR ;
+                  PAIR
+                } ;
+           PAIR}%michelson.
+
+
+Definition slc_ep_transfer :
+  instruction_seq (Some (parameter_ty, None)) false
+                  (parameter_transfer_ty ::: storage_context_ty ::: storage_auth_ty ::: nil)
+                  (list operation ::: storage_context_ty ::: storage_auth_ty ::: nil)
+  := slc_ep_transfer1_check_signature ;;;
+     { slc_ep_transfer2_transaction_iter ;
+       slc_ep_transfer3_register }.
+
+Definition slc_ep_receive :
+  instruction_seq (Some (parameter_ty, None)) false
+              (unit ::: storage_context_ty ::: storage_auth_ty ::: nil)
+              (list operation ::: storage_context_ty ::: storage_auth_ty ::: nil)
+  := { DROP1 ; (* cas d'un simple ajout de fonds (parameter : (Left Unit)) *)
+       NIL operation }%michelson.
+
+Definition dsl :
+  instruction_seq _ _
+              (pair parameter_ty storage_ty ::: nil)
+              (pair (list operation) storage_ty ::: nil)
+  :=
+    { UNPAPAIR ;
+      IF_RIGHT { (* cas d'un appel par la clef maîtresse *)
+          IF_LEFT
+            slc_ep_master
+            slc_ep_transfer
+        }
+               slc_ep_receive ;
+      PAPAIR}%michelson.
+
+Definition slc_contract_file : contract_file :=
+  Mk_contract_file parameter_ty None storage_ty Datatypes.false dsl.
+
+End Spending_limit_contract_definition.
