src/contracts_coq/spending_limit_contract_parsing.v
@@ -1,0 +1,59 @@
+(* Open Source License *)
+(* Copyright (c) 2019 Nomadic Labs. <contact@nomadic-labs.com> *)
+
+(* Permission is hereby granted, free of charge, to any person obtaining a *)
+(* copy of this software and associated documentation files (the "Software"), *)
+(* to deal in the Software without restriction, including without limitation *)
+(* the rights to use, copy, modify, merge, publish, distribute, sublicense, *)
+(* and/or sell copies of the Software, and to permit persons to whom the *)
+(* Software is furnished to do so, subject to the following conditions: *)
+
+(* The above copyright notice and this permission notice shall be included *)
+(* in all copies or substantial portions of the Software. *)
+
+(* THE SOFTWARE IS PROVIDED "AS IS", WITHOUT WARRANTY OF ANY KIND, EXPRESS OR *)
+(* IMPLIED, INCLUDING BUT NOT LIMITED TO THE WARRANTIES OF MERCHANTABILITY, *)
+(* FITNESS FOR A PARTICULAR PURPOSE AND NONINFRINGEMENT. IN NO EVENT SHALL *)
+(* THE AUTHORS OR COPYRIGHT HOLDERS BE LIABLE FOR ANY CLAIM, DAMAGES OR OTHER *)
+(* LIABILITY, WHETHER IN AN ACTION OF CONTRACT, TORT OR OTHERWISE, ARISING *)
+(* FROM, OUT OF OR IN CONNECTION WITH THE SOFTWARE OR THE USE OR OTHER *)
+(* DEALINGS IN THE SOFTWARE. *)
+
+Require Import main syntax_type syntax.
+
+Require Import spending_limit_contract_string String.
+
+Definition slc_contract_file_m := main.contract_file_M slc_contract 500.
+Definition slc_contract_file_m' := main.print_info slc_contract 500.
+
+Fact slc_contract_well_parsed :  error.is_true (error.success slc_contract_file_m).
+Proof. exact I. Defined.
+
+Definition dsl_contract_file := Eval cbv in (error.extract slc_contract_file_m slc_contract_well_parsed ).
+
+Require Import spending_limit_contract_definition.
+
+Module SLC_equiv.
+
+  Module slc_def := Spending_limit_contract_definition dummy_contract_context.
+
+  Definition slc_contract_file : syntax.contract_file :=
+    syntax.Mk_contract_file parameter_ty
+                            None
+                            storage_ty
+                            Datatypes.false
+                            slc_def.dsl.
+
+  Definition dsl_parameter := Eval cbv in syntax.contract_file_parameter dsl_contract_file.
+
+  (* Problem: different parameter types because of ignored annotations *)
+  Fact dsl_parameter_is_not_parameter_ty :
+    slc_def.slc_contract_file <> dsl_contract_file.
+  Proof.
+    intro H.
+    injection H.
+    intros.
+    discriminate.
+  Qed.
+
+End SLC_equiv.
