src/contracts_coq/spending_limit_contract_verification.v
@@ -1,0 +1,1138 @@
+Require Import String ZArith.
+Require Import syntax macros semantics comparable util.
+Import error.
+Require List.
+Require tez.
+Require map.
+
+Require List.
+Import List.ListNotations.
+Open Scope list.
+
+Require Import spending_limit_contract_definition.
+
+Module Spending_limit_contract_verification (C:ContractContext).
+
+Module slc_def := Spending_limit_contract_definition C.
+Import slc_def.
+
+Module semantics := Semantics C. Import semantics.
+
+
+Module Tactics.
+  (*
+   * Solves some fuel-related goals on the form
+   *   Hfuel : Y <= fuel |- X <= fuel by showing X <= Y
+   *)
+  Hint Rewrite List.rev_length : fuel.
+
+  Ltac simple_fuel :=
+    match goal with
+    | Hfuel:_ <= ?fuel |- _ =>
+      autorewrite with fuel in *;
+      apply (le_trans_rev _ _ _ Hfuel); simpl; omega
+    end.
+
+  (* Tactics for rewriting under existential binders *)
+  Ltac ex_under_aux' tac := etransitivity; [eapply forall_ex; intro; tac; apply iff_refl|].
+  Ltac ex_under_aux tac :=  ex_under_aux' tac || (rewrite iff_comm; ex_under_aux' tac; rewrite iff_comm).
+  Tactic Notation "ex_under" tactic(T) := ex_under_aux ltac:(T).
+  Ltac ex_rewrite rw := ex_under_aux ltac:(rewrite rw).
+
+
+
+  Ltac S_fuel_to_add_fuel  :=
+    match goal with
+    | [ fuel : Datatypes.nat |- _ ] =>
+      repeat match goal with
+             | [ |- context[S fuel] ] => change (S fuel) with (1 + fuel)
+             | [ |- context[S (?n + fuel)] ] => change (S (n + fuel)) with ((S n) + fuel)
+             end
+    end.
+
+  Ltac simple_fuel_add_n_fuel :=
+    match goal with
+    | [ fuel : Datatypes.nat |- _ ] =>
+      match goal with
+      | [ |- ?n <= ?m + fuel ] => apply Nat.le_sub_le_add_l
+      end
+    end.
+
+  Ltac my_simple_fuel :=
+    intros; try S_fuel_to_add_fuel; try simple_fuel_add_n_fuel;
+    (omega || simple_fuel).
+
+  Lemma my_simple_fuel_test_1:
+    forall (A : type) (xs : Datatypes.list (data A)) (fuel : Datatypes.nat),
+      Datatypes.length xs <= fuel ->
+      1 + Datatypes.length xs <= S fuel.
+  Proof. my_simple_fuel. Qed.
+
+  Lemma my_simple_fuel_test_2:
+    forall (fuel : Datatypes.nat) (L : Datatypes.list (comparable_data timestamp * comparable_data mutez)),
+      1 + Datatypes.length L <= fuel -> 1 + Datatypes.length L <= fuel.
+  Proof.
+    intros fuel L H.
+    my_simple_fuel.
+  Qed.
+End Tactics.
+
+Import Tactics.
+
+Fixpoint total_amount_transaction_list1
+         (transaction_list : (data (list (pair mutez (contract unit)))))
+         (acc : data mutez)
+         (result : data mutez) : Prop :=
+  match transaction_list with
+  | nil => result = acc
+  | cons (tz, _) transaction_list =>
+    exists new_acc,
+    (add _ _ _ Add_variant_tez_tez acc tz) = Return new_acc  /\
+    (total_amount_transaction_list1 transaction_list new_acc result)
+  end.
+
+Definition total_amount_transaction_list
+           (transaction_list : data (list (pair mutez (contract unit))))
+           (result : data mutez) :=
+  total_amount_transaction_list1 transaction_list (0 ~Mutez) result.
+
+Definition slc_ep_transfer2_transaction_iter_body_spec {A} env :
+      (stack (list operation ::: mutez ::: A) -> Prop) ->
+      (data (pair mutez (contract unit))) ->
+      stack (list operation ::: mutez ::: A) -> Prop :=
+  fun psi '(transferred_amount, destination) '(oplist, (threshold, st)) =>
+    exists new_threshold,
+    add _ _ _ Add_variant_tez_tez threshold transferred_amount = Return new_threshold /\
+    psi ((transfer_tokens (self_ty := Some (parameter_ty, None)) env unit tt transferred_amount destination) :: oplist,
+         (new_threshold, st)).
+
+Lemma slc_ep_transfer2_transaction_iter_body_spec_precond_ex A env psi transferred_amount destination oplist threshold st :
+  slc_ep_transfer2_transaction_iter_body_spec (A := A) env psi (transferred_amount, destination) (oplist, (threshold, st)) =
+  precond_ex (add _ _ _ Add_variant_tez_tez threshold transferred_amount)
+             (fun new_threshold => psi ((transfer_tokens (self_ty := Some (parameter_ty, None)) env unit tt transferred_amount destination) :: oplist,
+                                        (new_threshold, st))).
+Proof.
+  reflexivity.
+Qed.
+
+Opaque add.
+Opaque sub.
+
+Lemma slc_ep_transfer2_transaction_iter_body_correct {A} env fuel :
+  forall (psi : stack (list operation ::: mutez ::: A) -> Prop)
+         (element : data (pair mutez (contract unit)))
+         (st : stack (list operation ::: mutez ::: A)),
+  7 <= fuel ->
+  eval_seq_precond fuel env slc_ep_transfer2_transaction_iter_body
+               psi
+               (element, st) <->
+  slc_ep_transfer2_transaction_iter_body_spec env
+    psi element st.
+Proof.
+  intros psi (transferred_amount, destination) (oplist, (threshold, st)) Hfuel.
+  rewrite slc_ep_transfer2_transaction_iter_body_spec_precond_ex.
+  rewrite <- precond_exists.
+  unfold slc_ep_transfer2_transaction_iter_body.
+  unfold eval_seq_precond.
+  simpl eval_seq_precond_body.
+  more_fuel.
+  simpl.
+  more_fuel.
+  simpl.
+  more_fuel.
+  simpl.
+  reflexivity.
+Qed.
+
+Lemma slc_ep_transfer2_transaction_iter_correct
+      {A}
+      env
+      psi
+      (transaction_list : data (list (pair mutez (contract unit))))
+      (st : stack A) :
+  forall
+    (oplist : data (list operation))
+    fuel
+    (threshold : data mutez),
+    50 + Datatypes.length transaction_list <= fuel ->
+    eval_precond fuel env (ITER (i := iter_list _) slc_ep_transfer2_transaction_iter_body) psi
+                 (transaction_list, (oplist, (threshold, st))) <->
+    exists final_threshold,
+      total_amount_transaction_list1 transaction_list threshold final_threshold /\
+      psi
+        (List.rev
+           (List.map
+              (fun '(transfered_amount, destination) =>
+                 transfer_tokens env unit tt transfered_amount destination) transaction_list) ++
+           oplist,
+         (final_threshold, st)).
+Proof.
+
+  intros oplist fuel threshold H.
+  rewrite <- eval_precond_correct.
+  rewrite precond_iter_bounded
+          with (body_spec := slc_ep_transfer2_transaction_iter_body_spec env)
+               (fuel_bound := 7).
+  - generalize dependent oplist.
+    generalize dependent threshold.
+    induction transaction_list as [| (head_mut, ct) transaction_list_tail ]; intros threshold oplist.
+    + rewrite iff_comm. apply ex_eq_simpl.
+    + simpl.
+      rewrite ex_2. rewrite ex_order.
+      apply forall_ex.
+      intro acc.
+      rewrite underex_and_assoc.
+      rewrite <- ex_and_comm.
+      apply and_both.
+      rewrite IHtransaction_list_tail; try my_simple_fuel.
+      rewrite <- List.app_assoc.
+      reflexivity.
+
+  - intros fuel0 (transferred_amount, destination) (oplist', (threshold', st')) psi0 Hfuel.
+    rewrite eval_seq_precond_correct.
+    apply slc_ep_transfer2_transaction_iter_body_correct.
+    assumption.
+
+  - intros psi1 psi2 (transferred_amount, destination) (oplist', (threshold', st')) Hpsi.
+    unfold slc_ep_transfer2_transaction_iter_body_spec.
+    apply forall_ex. intro new_threshold. rewrite Hpsi. reflexivity.
+
+  - simple_fuel.
+Qed.
+Definition reverse {sty A B} :
+  instruction
+    sty false
+    (list A ::: list A ::: B)
+    (list A ::: B)
+  := ITER (i := iter_list _) { CONS }.
+
+
+Definition reverse_body_spec
+           {A : type} {B : Datatypes.list type}
+           (psi : stack (list A ::: B) -> Prop)
+           (x : data A)
+           (st : stack (list A ::: B)) : Prop :=
+  match st with
+    (xs, st') => psi (cons x xs, st')
+  end.
+
+Lemma reverse_correct
+      fuel self_type env (A : type) (B : Datatypes.list type)
+      (xs ys : data (list A))
+      (st : stack B)
+      (psi : stack (list A ::: B) -> Prop) :
+    2 + Datatypes.length xs <= fuel ->
+    eval_precond (self_type := self_type) fuel env reverse psi (xs, (ys, st))
+    <-> psi (List.app (List.rev xs) ys, st).
+Proof.
+  intros Hfuel.
+  extract_fuel (Datatypes.length xs + 1).
+  rewrite <- Nat.add_assoc.
+  rewrite <- eval_precond_correct.
+  unfold reverse.
+  rewrite precond_iter_bounded with
+      (body_spec := reverse_body_spec)
+      (fuel_bound := 1).
+  rewrite fold_right_psi_simpl with
+      (f := reverse_body_spec)
+      (f' := fun x '(ys, st)  => (cons x ys, st)).
+  - apply eq_iff_refl.
+    f_equal.
+    fold data.
+    generalize (@List.rev (data A) xs) ys.
+    induction l; intro ys'; simpl.
+    + reflexivity.
+    + now rewrite IHl.
+  - destruct st0. reflexivity.
+  - intros fuel0 x (xs', st') psi0 H.
+    more_fuel. simpl. reflexivity.
+  - intros psi1 psi2 x (xs', st') H.
+    apply H.
+  - omega.
+Qed.
+
+Definition slc_ep_transfer_loop_body_spec self_type (env : @proto_env self_type)
+           (input : stack (list (pair timestamp mutez) ::: list (pair timestamp mutez) ::: mutez ::: storage_auth_ty ::: nil))
+           (*
+            * (output : stack (bool ::: list (pair timestamp mutez) ::: list (pair timestamp mutez) ::: mutez ::: storage_auth_ty ::: nil))
+            *)
+           psi : Prop :=
+  let '(q1, (q2, (amount, st))) := input in
+  match q1, q2 with
+    | hd :: q1', q2 =>
+      if ((fst hd) <=? (now env))%Z
+      then exists sum, add _ _ _ Add_variant_tez_tez amount (snd hd) = Return sum /\
+                       psi (true, (q1', (q2, (sum, st))))
+      else psi (false, (q1, (q2, (amount, st))))
+    | [], hd :: q2' => psi (true, (List.rev (hd :: q2'), ([], (amount, st))))
+    | [], [] => psi (false, ([], ([], (amount, st))))
+  end.
+
+Lemma slc_ep_transfer_loop_body_correct env fuel psi (q1 q2 : data (list (pair timestamp mutez))) amount st :
+  (* sum (queue) + amount = init_thresh *)
+  30 + Datatypes.length q2 * 14 <= fuel ->
+  eval_precond fuel  env slc_ep_transfer_loop_body psi (q1, (q2, (amount, st)))
+  <-> slc_ep_transfer_loop_body_spec _ env (q1, (q2, (amount, st))) psi.
+Proof.
+  intros Hfuel.
+  unfold slc_ep_transfer_loop_body.
+  simpl.
+  destruct q1; simpl.
+  - destruct q2; simpl.
+    + now (do 5 more_fuel; simpl).
+    + simpl in Hfuel.
+      more_fuel; simpl.
+      more_fuel; simpl.
+      more_fuel; simpl.
+      destruct q2; [reflexivity|].
+      match goal with |- context[eval_precond fuel env (@ITER ?st ?c ?i ?A ?code) ?psi] =>
+                      remember (eval_precond fuel env (@ITER st c i A code) psi) as eval_itercode
+      end.
+      more_fuel.
+      simpl eval_precond.
+      subst eval_itercode.
+      rewrite reverse_correct; [|my_simple_fuel].
+      simpl.
+      rewrite <- List.app_assoc.
+      reflexivity.
+  - destruct d as (ts, tz).
+    do 6 (more_fuel; simpl).
+    rewrite <- comparison_to_int_leb.
+    rewrite <- comparison_to_int_opp.
+    destruct (_ >=? _)%Z.
+    + rewrite precond_exists. simpl. unfold precond_ex.
+      apply forall_ex.
+      intro x.
+      apply and_both_0; [|reflexivity].
+      rewrite add_comm; reflexivity.
+    + reflexivity.
+Qed.
+
+(* Start defining specification *)
+
+Fixpoint allowed_amount l rem now result :=
+  match l with
+  | nil => result = rem
+  | cons (frozen_timestamp, frozen_amount) l =>
+    match compare timestamp frozen_timestamp now with
+    (* Modified Arvid & Zaynah *)
+    (* frozen_timestamp <= now *)
+    | Lt | Eq =>
+           exists new_rem,
+           (* new_rem = rem + frozen_amount *)
+           add _ _ _ Add_variant_tez_tez rem frozen_amount = Return new_rem /\
+           allowed_amount l new_rem now result
+    | Gt => result = rem
+    end
+  end.
+
+(* true iff exists t1 \in l1, t1 > now *)
+Fixpoint queue_cut_before_now (l1 : data (list (pair timestamp mutez))) (now : data timestamp) : Datatypes.bool :=
+  match l1 with
+  | nil => false
+  | cons (t, _) l1 =>
+    match compare timestamp t now with
+    (* t <= now *)
+    | Lt | Eq => queue_cut_before_now l1 now
+    | Gt => true
+    end
+  end.
+
+(* filter (fun ts => ts > now) l *)
+Fixpoint remove_past (l : data (list (pair timestamp mutez))) (now : data timestamp) :=
+  match l with
+  | nil => nil
+  | cons (t, m) l =>
+    match compare timestamp t now with
+    | Lt | Eq => remove_past l now
+    | Gt => (t,m)::l
+    end
+  end.
+
+Definition update_queue l1 l2 now :=
+  if queue_cut_before_now l1 now then
+    (remove_past l1 now, l2)
+  else
+    (* l1 can be removed completely *)
+    (remove_past (List.rev l2) now, nil).
+
+Lemma slc_ep_transfer_loop_correct1
+      env
+      fuel
+      psi
+      (q1 q2 : data (list (pair timestamp mutez)))
+      (amount : data mutez)
+      (st : stack (storage_auth_ty ::: nil)) :
+  Datatypes.length q1 * 14 + Datatypes.length q2 * 14 + 48 <= fuel ->
+  queue_cut_before_now q1 (now env) = true ->
+  eval_precond  fuel env slc_ep_transfer_loop psi (true, (q1, (q2, (amount, st)))) <->
+  (exists amount' ,
+      allowed_amount q1 amount (now env) amount' /\
+      psi (remove_past q1 (now env), (q2, (amount', st)))).
+Proof.
+  intros Hfuel Hqueue_cut.
+
+  unfold slc_ep_transfer_loop.
+
+  generalize dependent amount.
+  generalize dependent fuel.
+  induction q1 as [ | (tz, ts) q1 ]; intros fuel Hfuel amount.
+
+  - inversion Hqueue_cut.
+  - rewrite plus_comm in Hfuel.
+    more_fuel; simpl.
+    rewrite slc_ep_transfer_loop_body_correct by my_simple_fuel.
+    unfold slc_ep_transfer_loop_body_spec.
+    unfold queue_cut_before_now in Hqueue_cut.
+    fold queue_cut_before_now in Hqueue_cut.
+
+    simpl compare in Hqueue_cut.
+    rewrite Z.leb_compare.
+    simpl fst.
+
+    unfold allowed_amount. simpl compare. fold allowed_amount.
+    unfold remove_past. simpl compare. fold remove_past.
+
+    repeat rewrite Z_match_compare_gt in *.
+
+    ex_rewrite Z_match_compare_gt.
+    destruct (now env <? tz)%Z eqn:HtzCompNow.
+
+    + more_fuel. simpl. rewrite iff_comm. apply ex_eq_simpl.
+
+    + rewrite ex_2. rewrite ex_order. apply forall_ex. intro sum.
+      rewrite underex_and_assoc. rewrite <- ex_and_comm. apply and_both.
+
+      now rewrite IHq1; try assumption; try my_simple_fuel.
+Qed.
+
+Lemma queue_cut_before_false_tl:
+ forall q a t x,
+  queue_cut_before_now ((a,t) :: q) x = false ->
+  queue_cut_before_now q x = false /\ (a <=? x)%Z = true.
+Proof.
+ simpl; intros; simpl in H.
+ rewrite  Z.leb_compare.
+ (*Set Printing All.*)
+ case_eq ((a ?= x)%Z ) ; intros; try rewrite H0 in H; simpl in H; try congruence; intuition.
+Qed.
+
+Remark add_mul: forall a b, 2* (S a) + b = a + (S (S a)) + b.
+Proof.
+  intros;omega.
+Qed.
+
+Lemma eval_precond_loop fuel self_ty (env : @proto_env self_ty) A (code : instruction _ false A (bool ::: A)) st psi :
+  eval_precond (S fuel) env (LOOP {code})%michelson psi (true, st) =
+  eval_precond fuel env code (eval_precond fuel env (LOOP {code})%michelson psi) st.
+Proof.
+  reflexivity.
+Qed.
+
+Lemma slc_ep_transfer_loop_correct2':
+  forall
+    env
+    psi
+    (q1 : data (list (pair timestamp mutez)))
+    fuel (x: data (pair timestamp mutez))
+    (q2 : data (list (pair timestamp mutez)))
+    ( Hfuel: 50 + Datatypes.length q2 * 14 <= fuel)
+    (Hqueue_cut : queue_cut_before_now (x::q1) (now env) = false)
+    (amount : data mutez)
+    (st : stack (storage_auth_ty ::: nil)),
+    eval_precond ((S (Datatypes.length q1)) + fuel) env slc_ep_transfer_loop psi (true, ((x::q1), (q2, (amount, st)))) <->
+    exists amount',
+      allowed_amount (x::q1) amount (now env) amount' /\
+      eval_precond fuel env slc_ep_transfer_loop
+                   psi ( true, ([],(q2, (amount',st)))).
+Proof.
+  intros env psi ; unfold slc_ep_transfer_loop. induction  q1 as [ | (tz, ts) q1 ]; intros.
+
+(* case q1 == nil *)
+  - destruct x.
+    simpl.
+    rewrite slc_ep_transfer_loop_body_correct by my_simple_fuel. simpl.
+    simpl in Hqueue_cut.
+    case_eq ( (d ?= now env)%Z); intros K; rewrite K in Hqueue_cut; inversion Hqueue_cut.
+    +  rewrite Z.leb_compare. rewrite K. intuition.
+     *  destruct H as [sum [Heq Prd]].
+        exists sum. split;auto.
+        exists sum. split;auto.
+
+
+     *  destruct H as [am [A Prd]].
+        destruct A as [sum' [Heq1 Heq2]].
+        subst. exists sum'.  split;auto.
+
+    + rewrite Z.leb_compare. rewrite K. intuition.
+      * destruct H as [sum [Heq Prd]].
+
+        exists sum. split;auto.
+        exists sum. split;auto.
+
+      * destruct H as [am [A Prd]].
+        destruct A as [sum' [Heq1 Heq2]].
+        subst. exists sum'.  split;auto.
+
+(* case q1 <> nil *)
+  - assert (Hqueue_ind: queue_cut_before_now ((tz, ts) :: q1) (now env) = false).
+    simpl in Hqueue_cut.
+    destruct x. case_eq ((d ?= now env)%Z  ); intro K; rewrite K in Hqueue_cut; inversion Hqueue_cut; auto.
+    simpl "+".
+    rewrite eval_precond_loop.
+     rewrite slc_ep_transfer_loop_body_correct. simpl.
+     destruct x. simpl. assert (Cond : (d <=? now env)%Z = true).
+     destruct (queue_cut_before_false_tl _ _ _ _ Hqueue_cut) as [A B]. auto.
+     rewrite Z.leb_compare. rewrite Z.leb_compare in Cond.
+     case_eq ( (d ?= now env)%Z); intros K ; rewrite K in Cond; inversion Cond ; try rewrite K.
+    + (* K : (d ?= now env)%Z = Eq *)
+      split.
+      *
+       intros [sum [Heq1 Prd]].
+       destruct (IHq1 fuel (tz,ts) q2 Hfuel Hqueue_ind sum st) as [Ia Ib].
+       destruct (Ia Prd) as [am [Alw Prd']].
+       exists am.  split;intuition. exists sum. split. auto.
+       simpl in Alw. auto.
+
+      *
+       intros [am [A Prd]]. destruct A as [sum [ Heq  Alw]].
+       exists sum. split. auto.
+       destruct (IHq1 fuel (tz,ts) q2 Hfuel Hqueue_ind sum st) as [Ia Ib].
+       apply Ib. exists am.  split; auto.
+    + (*K : (d ?= now env)%Z = Lt*)
+      split.
+      *
+       intros [sum [Heq1 Prd]].
+       destruct (IHq1 fuel (tz,ts) q2 Hfuel Hqueue_ind sum st) as [Ia Ib].
+       destruct (Ia Prd) as [am [Alw Prd']].
+       exists am.  split;intuition. exists sum. split. auto.
+       simpl in Alw. auto.
+      *
+       intros [am [A Prd]]. destruct A as [sum [ Heq  Alw]].
+       exists sum. split. auto.
+       destruct (IHq1 fuel (tz,ts) q2 Hfuel Hqueue_ind sum st) as [Ia Ib].
+       apply Ib. exists am.  split; auto.
+    + 
+   (* fuel bound *)
+    apply le_trans with (50 +Datatypes.length q2 * 14); omega.
+Qed.
+
+(*****************************************************************)
+
+Definition list_empty_b (q2 : data (list (pair timestamp mutez))) : Datatypes.bool :=
+  match q2 with nil => true | _ => false end.
+
+
+(* probably not used *)
+Lemma slc_ep_transfer_loop_correct3'
+      env
+      fuel
+      psi
+      (q2 : data (list (pair timestamp mutez)))
+      (amount : data mutez)
+      (st : stack (storage_auth_ty ::: nil)) :
+  50 + Datatypes.length q2 * 14 <= fuel ->
+  (eval_precond (S fuel) env slc_ep_transfer_loop psi (true, ([], (q2, (amount, st)))) <->
+   eval_precond fuel env slc_ep_transfer_loop psi (negb (list_empty_b q2), (List.rev q2, ([], (amount, st))))).
+Proof.
+  intros Hfuel.
+  simpl.
+  rewrite slc_ep_transfer_loop_body_correct by my_simple_fuel.
+  simpl slc_ep_transfer_loop_body_spec.
+  unfold slc_ep_transfer_loop.
+  destruct q2; reflexivity.
+Qed.
+
+Lemma slc_ep_transfer_loop_correct3
+      env
+      fuel
+      psi
+      (x : data (pair timestamp mutez))
+      (q2 : data (list (pair timestamp mutez)))
+      (amount : data mutez)
+      (st : stack (storage_auth_ty ::: nil)) :
+  50 + Datatypes.length q2 * 14 <= fuel ->
+  (eval_precond (S fuel) env slc_ep_transfer_loop psi (true, ([], (x :: q2, (amount, st)))) <->
+   eval_precond fuel env slc_ep_transfer_loop psi (true, (List.rev (x :: q2), ([], (amount, st))))).
+Proof.
+  intros Hfuel. simpl.
+  rewrite slc_ep_transfer_loop_body_correct by my_simple_fuel.
+  reflexivity.
+Qed.
+
+Lemma slc_ep_transfer_loop_correct4
+      env
+      fuel
+      psi
+      (amount : data mutez)
+      (st : stack (storage_auth_ty ::: nil)) :
+  50 <= fuel ->
+  (eval_precond fuel env slc_ep_transfer_loop psi (false, ([], ([], (amount, st)))) <->
+   psi (([], ([], (amount, st))))).
+Proof.
+  intros Hfuel. do 2 more_fuel. simpl. intuition.
+Qed.
+
+Lemma slc_ep_transfer_loop_correct2
+      env
+      fuel
+      psi
+      (q1 q2 : data (list (pair timestamp mutez)))
+      (amount : data mutez)
+      (st : stack (storage_auth_ty ::: nil)) :
+      50 + Datatypes.length q1 * 14 + Datatypes.length q2 * 14 <= fuel ->
+      queue_cut_before_now q1 (now env) = false ->
+      eval_precond (Datatypes.length q1 + 1 + fuel) env slc_ep_transfer_loop
+                   psi (true, (q1, (q2, (amount, st)))) <->
+      exists amount',
+        allowed_amount q1 amount (now env) amount' /\
+        eval_precond fuel env slc_ep_transfer_loop
+                     psi (negb (list_empty_b q2), (List.rev q2,([], (amount',st)))).
+Proof.
+  intros Hfuel Hqueue_cut.
+  destruct q1.
+  - simpl (Datatypes.length _ + 1 + fuel).
+    rewrite slc_ep_transfer_loop_correct3'.
+    + simpl.
+      rewrite ex_eq_simpl.
+      destruct q2; more_fuel; reflexivity.
+    + assumption.
+
+  - simpl Datatypes.length.
+    rewrite <- Nat.add_assoc.
+    replace (2 + fuel) with (S (S fuel)) by omega.
+    rewrite slc_ep_transfer_loop_correct2'; try my_simple_fuel; try assumption.
+    apply forall_ex. intro amount'.
+    now rewrite slc_ep_transfer_loop_correct3' by my_simple_fuel.
+Qed.
+
+Lemma queue_cut_before_now_allowed_amount :
+  forall (q1 q2 : (data (list (pair timestamp mutez)))) ts tresh1 tresh,
+    queue_cut_before_now q1 ts = true ->
+    allowed_amount (q1 ++ q2) tresh ts tresh1 <-> allowed_amount q1 tresh ts tresh1.
+Proof.
+  intros q1 q2 ts tresh1.
+
+  induction q1.
+  + now simpl.
+  + destruct a as (ts0, tz).
+    rewrite <- List.app_comm_cons.
+    simpl.
+
+    intros tresh H.
+    repeat rewrite Z_match_compare_gt in *.
+
+    destruct ((ts <? ts0)%Z).
+    * intuition.
+    * apply forall_ex. intro new_rem. now rewrite IHq1.
+Qed.
+
+Lemma remove_past_no_now :
+  forall q n,
+    queue_cut_before_now q n = false ->
+    remove_past q n = [].
+Proof. simpl. intros.
+       induction q. now simpl.
+       destruct a.
+       simpl in *.
+       destruct (z ?= n)%Z; auto.
+       inversion H.
+Qed.
+
+Lemma update_queue_not_in  :
+  forall q1 q2 ts,
+    queue_cut_before_now q1 ts = false ->
+    update_queue q1 q2 ts =
+    update_queue (List.rev q2) [] ts.
+Proof.
+  simpl. intros q1 q2 ts H. unfold update_queue.
+  rewrite H.
+  destruct (queue_cut_before_now (List.rev q2) ts) eqn:HqueueCut.
+  reflexivity.
+  simpl.
+  now rewrite remove_past_no_now.
+Qed.
+
+Lemma Hupdate_queue_no_now self_ty (env : @proto_env self_ty):
+  forall (q1 q2 : data (list (pair timestamp mutez))),
+    queue_cut_before_now q1 (now env) = false ->
+    queue_cut_before_now (List.rev q2) (now env) = false ->
+    ([], []) = update_queue q1 q2 (now env).
+Proof.
+  intros q1 q2 Hq1 Hq2.
+  unfold update_queue. rewrite Hq1.
+  now rewrite remove_past_no_now.
+Qed.
+
+Lemma allowed_amount_app1 :
+  forall q1 ts0 a a1 a2 q2,
+    queue_cut_before_now q1 ts0 = false ->
+    allowed_amount q1 a ts0 a1 ->
+    allowed_amount q2 a1 ts0 a2 ->
+    allowed_amount (q1 ++ q2) a ts0 a2.
+Proof.
+  simpl. intros q1.
+  induction q1 as [|(ts,mt)]; intros ts0 a a1 a2 q2.
+  - simpl. intuition congruence.
+  - rewrite <- List.app_comm_cons.
+    simpl.
+    repeat rewrite Z_match_compare_gt.
+    destruct ((ts0 <? ts)%Z) eqn:Heq; [intro H; inversion H|].
+    intros Hsort [a1' [Hadd1 Hq1']] Hq2.
+    exists a1'. intuition.
+    apply IHq1 with a1; assumption.
+Qed.
+
+Lemma allowed_amount_app2 :
+  forall q1 ts0 a a2 q2,
+    queue_cut_before_now q1 ts0 = false ->
+    allowed_amount (q1 ++ q2) a ts0 a2 ->
+    exists a1,
+      allowed_amount q1 a ts0 a1 /\
+      allowed_amount q2 a1 ts0 a2.
+Proof.
+  simpl. intros q1.
+  induction q1 as [|(ts,mt)].
+  - simpl. eauto.
+  - simpl.
+    intros ts0 a a2 q2.
+    repeat rewrite Z_match_compare_gt.
+    destruct (ts0 <? ts)%Z eqn:Hts0LtTs; [intro H; inversion H|].
+    intros Hqueue_cut [a' [Ha' Hallowed']].
+    specialize (IHq1 _ _ _ _ Hqueue_cut Hallowed') as [a1 [Hq1 Hq2]].
+    exists a1.
+    rewrite Z_match_compare_gt. rewrite Hts0LtTs. eauto.
+Qed.
+
+Lemma allowed_amount_app :
+  forall q1 ts0 a a2 q2,
+    queue_cut_before_now q1 ts0 = false ->
+    allowed_amount (q1 ++ q2) a ts0 a2 <->
+    exists a1,
+      allowed_amount q1 a ts0 a1 /\
+      allowed_amount q2 a1 ts0 a2.
+Proof.
+  simpl. split.
+  now apply allowed_amount_app2.
+  intros [a1 [Ha1 Ha1']].
+  now apply allowed_amount_app1 with a1.
+Qed.
+
+Lemma slc_ep_transfer_loop_correct
+      env
+      fuel
+      psi
+      (q1 q2 : data (list (pair timestamp mutez)))
+      (amount : data mutez)
+      (st : stack (storage_auth_ty ::: nil)) :
+  Datatypes.length q1 * 18 + Datatypes.length q2 * 16 + 54 <= fuel ->
+  eval_precond fuel env slc_ep_transfer_loop psi (true, (q1, (q2, (amount, st)))) <->
+  (exists (amount' : data mutez),
+      let (q1', q2') := update_queue q1 q2 (now env) in
+      allowed_amount (q1 ++ List.rev q2) amount (now env) amount' /\
+      psi (q1', (q2', (amount', st)))).
+Proof.
+  intros Hfuel.
+
+  destruct (queue_cut_before_now q1 (now env)) eqn:Hqueue.
+
+  (* If now is in q1 *)
+  - rewrite slc_ep_transfer_loop_correct1; try simple_fuel; try assumption.
+    unfold update_queue. rewrite Hqueue.
+    ex_under (rewrite queue_cut_before_now_allowed_amount at 1 by assumption).
+    reflexivity.
+
+  (* If now is not in q1 *)
+  - (* extract fuel *)
+    extract_fuel (Datatypes.length q1 + 1).
+
+    rewrite slc_ep_transfer_loop_correct2; try assumption; try simple_fuel.
+
+    destruct q2.
+
+    (* if q2 is empty *)
+    + rewrite update_queue_not_in by apply Hqueue. simpl.
+      rewrite List.app_nil_r.
+
+      apply forall_ex. intro amount'.
+      apply and_both.
+      apply slc_ep_transfer_loop_correct4; try simple_fuel.
+
+    (* if q2 is non-empty *)
+    + destruct (update_queue q1 (d :: q2) (now env)) eqn:Heq. simpl in l0.
+      ex_under (rewrite allowed_amount_app at 1 by assumption).
+      rewrite ex_2. rewrite ex_order. apply forall_ex; intro amount1.
+      rewrite underex_and_assoc. rewrite <- ex_and_comm. apply and_both.
+
+      unfold update_queue in Heq. rewrite Hqueue in Heq.
+      apply and_pair_eq in Heq as [Heq1 Heq2].
+      subst l. subst l0.
+
+      destruct (queue_cut_before_now (List.rev (d :: q2)) (now env)) eqn:HnowInQ2; try assumption.
+
+      (* If now is in (List.rev (d :: q2)) *)
+      * rewrite slc_ep_transfer_loop_correct1. reflexivity.
+        (* fuel arithmetic *)
+        simpl (Datatypes.length []). rewrite List.rev_length. simple_fuel.
+        assumption.
+
+      (* If now is not in (List.rev (d :: q2)) *)
+      * (* extract fuel *)
+        extract_fuel (Datatypes.length (List.rev (d :: q2)) + 1).
+
+        rewrite slc_ep_transfer_loop_correct2; [|my_simple_fuel|assumption].
+        apply forall_ex; intro amount'.
+        rewrite slc_ep_transfer_loop_correct4; [|my_simple_fuel].
+        rewrite remove_past_no_now by assumption.
+        reflexivity.
+
+        symmetry. apply le_plus_minus. my_simple_fuel.
+Qed.
+
+Definition sig_header_ty :=
+  (pair
+     (contract parameter_ty)
+     chain_id).
+
+Definition slc_ep_transfer1_check_signature_spec
+    (env : @proto_env (Some (parameter_ty, None)))
+    (fuel : Datatypes.nat)
+    (transactions : data (list (pair mutez (contract unit))))
+    (slave_key : data key)
+    (slave_signature : data signature)
+    (slave_key_hash new_slave_key_hash : data key_hash)
+    (time_limit : data int)
+    (queue_left queue_right : data (list (pair timestamp mutez)))
+    (threshold : data mutez)
+    (master_salt slave_salt : data nat)
+    (master_key_hash : data key_hash)
+    (psi : stack (list (pair mutez (contract unit)) :::
+                            list operation ::: mutez ::: key_hash ::: int ::: mutez ::: list (pair timestamp mutez) :::
+                            list (pair timestamp mutez) ::: storage_auth_ty ::: nil) -> Prop)
+  :=
+  hash_key env slave_key = slave_key_hash /\
+  check_signature env slave_key slave_signature
+                  (pack env (pair (list (pair mutez (contract unit))) key_hash) (transactions, new_slave_key_hash)
+                        ++ pack env sig_header_ty (self env None I, (chain_id_ env))
+                        ++ pack env nat slave_salt)%string = true /\
+  (exists (threshold_gc : data mutez) ,
+      let (q1', q2') := update_queue queue_left queue_right (now env) in
+      allowed_amount (queue_left ++ List.rev queue_right) threshold (now env) threshold_gc /\
+       psi
+              (transactions,
+               ([],
+                (0 ~Mutez,
+                 (new_slave_key_hash,
+                  (time_limit,
+                   (threshold_gc,
+                    (q1',
+                     (q2', ((master_key_hash, (master_salt, (slave_salt + 2)%N)), tt)))))))))).
+Transparent add.
+Opaque N.add.
+
+Lemma slc_ep_transfer1_check_signature_correct
+        (env : @proto_env (Some (parameter_ty, None)))
+        (transactions : data (list (pair mutez (contract unit))))
+        (slave_key : data key)
+        (slave_signature : data signature)
+        (slave_key_hash new_slave_key_hash : data key_hash)
+        (time_limit : data int)
+        (queue_left queue_right : data (list (pair timestamp mutez)))
+        (threshold : data mutez)
+        (master_salt slave_salt : data nat)
+        (master_key_hash : data key_hash)
+        (psi : stack (list (pair mutez (contract unit)) :::
+                         list operation ::: mutez ::: key_hash ::: int ::: mutez ::: list (pair timestamp mutez) :::
+                         list (pair timestamp mutez) ::: storage_auth_ty ::: nil) ->
+               Prop) :
+  forall fuel,
+    84 + Datatypes.length queue_left * 18 + Datatypes.length queue_right * 16 <= fuel ->
+    let params_transfer : data parameter_transfer_ty := ((transactions, new_slave_key_hash), (slave_key, slave_signature)) in
+    let storage_context : data storage_context_ty := (slave_key_hash, ((threshold, time_limit), (queue_left, queue_right))) in
+    let storage_auth : data storage_auth_ty := (master_key_hash, (master_salt, slave_salt)) in
+    eval_seq_precond (S (S (S (S (S (S (S fuel))))))) env (slc_ep_transfer1_check_signature)
+                 psi (params_transfer, (storage_context, (storage_auth, tt)))
+    <->
+    slc_ep_transfer1_check_signature_spec
+      env fuel transactions slave_key slave_signature slave_key_hash new_slave_key_hash
+      time_limit queue_left queue_right
+      threshold master_salt slave_salt master_key_hash
+      psi.
+Proof.
+  intros fuel Hfuel params_transfer storage_context storage_auth.
+  unfold slc_ep_transfer1_check_signature.
+  remember slc_ep_transfer_loop as transfer_loop.
+  rewrite <- plus_assoc in Hfuel.
+  do 30 more_fuel'.
+  unfold eval_seq_precond.
+  simpl.
+  repeat rewrite fold_eval_precond.
+  unfold slc_ep_transfer1_check_signature_spec.
+
+  rewrite match_if_exchange.
+  rewrite if_false_is_and.
+  rewrite (eqb_eq key_hash).
+
+  apply and_both_0.
+  apply eq_sym_iff.
+  rewrite match_if_exchange.
+  rewrite if_false_is_and.
+  apply and_both.
+
+  rewrite Heqtransfer_loop.
+  (* todo: rewrite precond (eval ) in lemmes to eval_precond *)
+  rewrite slc_ep_transfer_loop_correct.
+  apply forall_ex.
+  intro amount'.
+  destruct (update_queue queue_left queue_right (now env)) eqn:Hq1q2.
+  apply and_both.
+
+  rewrite N.add_comm.
+  reflexivity.
+
+  (* fuel stuff *)
+  my_simple_fuel.
+Qed.
+
+Lemma slc_ep_transfer3_register_correct
+      env
+      fuel
+      psi
+      (transaction_oplist : data (list operation))
+      (transaction_list_total : data mutez)
+      (new_slave_key_hash : data key_hash)
+      (time_limit : data int)
+      (threshold : data mutez)
+      (q1 q2 : data (list (pair timestamp mutez)))
+      (st : data storage_auth_ty) :
+  50 <= fuel ->
+  eval_precond fuel env slc_ep_transfer3_register
+                 psi
+                (transaction_oplist,
+                 (transaction_list_total,
+                  (new_slave_key_hash,
+                   (time_limit,
+                    (threshold,
+                     (q1, (q2, (st, tt)))))))) <->
+  exists new_threshold,
+    let new_storage_context : data storage_context_ty :=
+        (new_slave_key_hash,
+         ((new_threshold, time_limit),
+          (q1, ((now env + time_limit)%Z, transaction_list_total) :: q2))) in
+    sub _ _ _ Sub_variant_tez_tez threshold transaction_list_total = Return new_threshold /\
+    psi (transaction_oplist, (new_storage_context, (st, tt))).
+Proof.
+  intros Hfuel.
+  simpl.
+  do 14 (more_fuel; simpl eval_precond).
+  more_fuel.
+  simpl (eval_precond (S fuel) env SUB _). unfold eval_precond_body.
+  remember (fun SA : _ => _) as psi'.
+  do 9 (more_fuel; simpl eval_precond).
+  rewrite precond_exists.
+  now subst psi'.
+Qed.
+
+Open Scope string_scope.
+
+Definition slc_spec (env : @proto_env (Some (parameter_ty, None))) (fuel : Datatypes.nat) (input : data (pair parameter_ty storage_ty)) (output : data (pair (list operation) (storage_ty))) :=
+  let '(param, storage) := input in
+  let '(storage_context, (master_key_hash, (master_salt, slave_salt))) := storage in
+  let '(slave_key_hash, ((threshold, time_limit), (queue_left, queue_right))) := storage_context in
+  match param with
+  (* Entrypoint: Receive *)
+  | inl _ =>
+     output = (nil, storage)
+  (* Entrypoint:  Master *)
+  | (inr (inl ((master_key, master_signature), payload))) =>
+    hash_key env master_key = master_key_hash /\
+    (* Pre-condition 2: the signature is valid *)
+    check_signature env master_key master_signature
+                    (pack env payload_ty payload
+                          ++ pack env sig_header_ty (self env None I, (chain_id_ env))
+                          ++ pack env nat master_salt) = true /\
+    match payload with
+    | inl (new_storage_context, new_master_key_hash) =>
+      (* Install new storage *)
+      output = (nil, (new_storage_context, (new_master_key_hash, (master_salt + 2, slave_salt)%N)))
+    | inr (existT _ _ lam, new_master_key_hash) =>
+      (* Run lambda *)
+      precond (eval_seq (no_self env) lam fuel (tt, tt))
+              (fun '(operations, tt) =>
+                 output = (operations, (storage_context, (new_master_key_hash, (master_salt + 2, slave_salt)%N))))
+    end
+  (* Entry point: Transfer *)
+  | inr (inr ((transactions, new_slave_key_hash), (slave_key, slave_signature))) =>
+    hash_key env slave_key = slave_key_hash /\
+    check_signature env slave_key slave_signature
+                    (pack env (pair (list (pair mutez (contract unit))) key_hash) (transactions, new_slave_key_hash)
+                          ++ pack env sig_header_ty (self env None I, (chain_id_ env))
+                          ++ pack env nat slave_salt) = true /\
+    (exists spent_amount threshold_gc new_threshold,
+      (* sum(transactions) = amount *)
+      total_amount_transaction_list transactions spent_amount /\
+      (* allowed(queue, threshold, now) = threshold_gc *)
+      allowed_amount (List.app queue_left (List.rev queue_right)) threshold (now env) threshold_gc /\
+      (* new_threshold = threshold_gc - spent_amount *)
+      sub _ _ _ Sub_variant_tez_tez threshold_gc spent_amount = Return new_threshold /\
+      let new_operations : data (list operation) :=
+          List.rev (List.map
+                      (fun '(transfered_amount, destination) => transfer_tokens env unit tt transfered_amount destination)
+                      transactions) in
+      let new_queue :=
+          (let (l1', l2') := update_queue queue_left queue_right (now env) in
+           (l1', cons ((now env + time_limit)%Z, spent_amount) l2')) in
+      let new_context : data storage_context_ty :=
+          (new_slave_key_hash, ((new_threshold, time_limit), new_queue)) in
+      output = (new_operations, (new_context, (master_key_hash, (master_salt, (slave_salt + 2)%N)))))
+  end.
+
+Definition slc_fuel_bound (input : data (pair parameter_ty storage_ty)) :=
+    let '(param, storage) := input in
+    let '(storage_context, (master_key_hash, master_salt)) := storage in
+    let '(slave_key_hash, ((threshold, time_limit), (queue_left, queue_right))) := storage_context in
+    match param with
+      (* entry point: receive *)
+      | inl _ => 14
+      (* entry point: master *)
+      | inr (inl _) => 30
+      (* entry point: transfer *)
+      | inr (inr ((transactions, _), _)) => Datatypes.length transactions + Datatypes.length queue_left * 18 + Datatypes.length queue_right * 16 + 89
+    end.
+
+
+Lemma slc_ep_transfer_correct :
+  forall env (p3 : data parameter_transfer_ty) (slave_key_hash : data key_hash) (threshold : data mutez) (time_limit : data int)
+         (queue_left queue_right : data (list (pair timestamp mutez))) (master_key_hash : data key_hash) (master_salt slave_salt : data nat)
+         (output : data (pair (list operation) storage_ty)) (fuel : Datatypes.nat),
+    (let (d, _) := p3 in
+     let (transactions, _) := d in Datatypes.length transactions + Datatypes.length queue_left * 18 + Datatypes.length queue_right * 16 + 89) <=
+    fuel ->
+    eval_seq_precond (4 + fuel) env dsl (fun x : stack [pair (list operation) storage_ty] => x = (output, tt))
+                 (inr (inr p3), (slave_key_hash, (threshold, time_limit, (queue_left, queue_right)), (master_key_hash, (master_salt, slave_salt))), tt) <->
+    slc_spec env fuel
+             (inr (inr p3), (slave_key_hash, (threshold, time_limit, (queue_left, queue_right)), (master_key_hash, (master_salt, slave_salt))))
+             output.
+Proof.
+  intros env p3 slave_key_hash threshold time_limit queue_left queue_right master_key_hash master_salt slave_salt output fuel Hfuel.
+
+  unfold dsl.
+  remember slc_ep_transfer as prog.
+  destruct p3 as ((transactions, new_slave_key_hash), (slave_key, slave_signature)).
+  unfold eval_seq_precond.
+  rewrite Nat.add_comm in Hfuel.
+  simpl eval_seq_precond_body.
+  do 5 more_fuel'; simpl.
+  rewrite Nat.add_comm in Hfuel.
+  repeat rewrite fold_eval_precond.
+  rewrite Heqprog. unfold slc_ep_transfer.
+
+  rewrite Nat.add_comm in Hfuel.
+  change (@eval_seq_precond_body (@eval_precond ?fuel)) with (@eval_seq_precond fuel).
+  rewrite eval_seq_assoc.
+  rewrite slc_ep_transfer1_check_signature_correct; [| my_simple_fuel].
+  unfold slc_ep_transfer1_check_signature_spec.
+  unfold slc_spec.
+  apply and_both.
+  apply and_both.
+
+  destruct (update_queue queue_left queue_right (now env)) eqn:Hupdate_queue. simpl in l0.
+
+  rewrite ex_order.
+  apply forall_ex; intro threshold_gc.
+  unfold seq_aux.
+  change (eval_seq_precond ?fuel env (SEQ ?i1 ?i2) ?psi ?st) with (eval_precond fuel env i1 (eval_seq_precond fuel env i2 psi) st).
+  rewrite slc_ep_transfer2_transaction_iter_correct; [| my_simple_fuel].
+  unfold total_amount_transaction_list.
+  rewrite iff_comm.
+
+  rewrite <- underex2_and_comm at 1.
+  rewrite underex2_and_assoc.
+
+  rewrite <- ex2_and_comm.
+  apply and_both.
+
+  apply forall_ex; intro spent_sum.
+
+  rewrite underex_and_comm.
+  rewrite <- ex_and_comm at 1.
+  apply and_both.
+
+  change (eval_seq_precond ?fuel env (SEQ ?i1 ?i2) ?psi ?st) with (eval_precond fuel env i1 (eval_seq_precond fuel env i2 psi) st).
+  rewrite slc_ep_transfer3_register_correct; [| my_simple_fuel].
+
+  apply forall_ex; intro final_threshold.
+
+  apply and_both.
+  unfold eval_seq_precond; simpl.
+  rewrite and_pair_eq.
+  rewrite List.app_nil_r.
+  intuition.
+Qed.
+
+Lemma slc_ep_master_correct:
+  forall env (p2 : data parameter_master_ty) (slave_key_hash : data key_hash) (threshold : data mutez) (time_limit : data int)
+         (queue_left queue_right : data (list (pair timestamp mutez))) (master_key_hash : data key_hash) (master_salt slave_salt : data nat)
+         (output : data (pair (list operation) storage_ty)) (fuel : Datatypes.nat),
+    30 <= fuel ->
+    eval_seq_precond (4 + fuel) env dsl (fun x : stack [pair (list operation) storage_ty] => x = (output, tt))
+                 (inr (inl p2), (slave_key_hash, (threshold, time_limit, (queue_left, queue_right)), (master_key_hash, (master_salt, slave_salt))), tt) <->
+    slc_spec env fuel
+             (inr (inl p2), (slave_key_hash, (threshold, time_limit, (queue_left, queue_right)), (master_key_hash, (master_salt, slave_salt))))
+             output.
+Proof.
+  intros env p2 slave_key_hash threshold time_limit queue_left queue_right master_key_hash master_salt slave_salt output fuel Hfuel.
+  destruct p2 as ((key, signature), payload).
+  unfold eval_seq_precond.
+  do 5 (more_fuel; simpl).
+  repeat rewrite fold_eval_precond.
+  rewrite match_if_exchange.
+  rewrite if_false_is_and.
+  rewrite (eqb_eq key_hash).
+  rewrite match_if_exchange.
+  rewrite if_false_is_and.
+  unfold slc_spec. rewrite N.add_comm.
+
+  destruct payload as [ (foo, slave_key_hash') | ((lam_ff, lam), slave_key_hash') ].
+
+  + simpl. intuition; congruence.
+
+  + unfold slc_spec.
+
+    apply and_both_0. apply eq_sym_iff.
+    apply and_both.
+
+    change (@eval_seq_precond_body (@eval_precond ?fuel)) with (@eval_seq_precond fuel).
+    rewrite <- (eval_seq_precond_correct lam).
+    apply precond_eqv.
+    intros [st1 []].
+    intuition.
+    inversion H. f_equal.
+    rewrite H. reflexivity.
+Qed.
+
+Theorem slc_correct env input output :
+  forall fuel,
+    fuel >= slc_fuel_bound input ->
+    eval_seq env dsl (4 + fuel) (input, tt) = Return (output, tt) <->
+    slc_spec env fuel input output.
+Proof.
+  unfold ">=".
+  intros fuel Hfuel.
+  rewrite return_precond.
+  rewrite eval_seq_precond_correct.
+  destruct input as (param,
+                     ((slave_key_hash, ((threshold, time_limit), (queue_left, queue_right))),
+                        (master_key_hash, (master_salt, slave_salt)))).
+
+  destruct param as [ [] | [ p2 | p3 ] ]; simpl in Hfuel.
+
+  (* Entry point: receive *)
+  - unfold eval_seq_precond. more_fuel. simpl. intuition congruence.
+  (* Entry point : master call *)
+  - apply slc_ep_master_correct. apply Hfuel.
+  (* Entry point : transfer *)
+  - apply slc_ep_transfer_correct. apply Hfuel.
+Qed.
+
+End Spending_limit_contract_verification.
