src/michocoq/util.v
@@ -178,6 +178,42 @@ Proof.
 Qed.
 
 
+Lemma le_trans_rev : forall n m p : Datatypes.nat, m <= p -> n <= m -> n <= p.
+Proof.
+  intros n m p Hmp Hnm. apply le_trans with m. apply Hnm. apply Hmp.
+Qed.
+
+
+Lemma comparison_to_int_opp : forall z1 z2, (comparison_to_int (z2 ?= z1) >=? 0)%Z =
+                                            (comparison_to_int (z1 ?= z2) <=? 0)%Z.
+Proof.
+  intros z1 z2.
+  rewrite Z.compare_antisym.
+  destruct (z1 ?= z2)%Z; simpl; tauto.
+Qed.
+
+Lemma Z_match_compare_gt :
+  forall A ts ts0 (x y : A),
+    match (ts ?= ts0)%Z with
+    | Gt => x
+    | _ => y
+    end =
+    if (ts0 <? ts)%Z then x else y.
+Proof.
+  intros A ts ts0 P Q.
+  rewrite Z.ltb_compare.
+  rewrite Z.compare_antisym.
+  destruct (ts0 ?= ts)%Z; simpl; reflexivity.
+Qed.
+
+Lemma comparison_to_int_leb :
+  forall z1 z2, (comparison_to_int (z1 ?= z2) <=? 0)%Z = (z1 <=? z2)%Z.
+Proof.
+  intros z1 z2.
+  repeat rewrite Z.leb_compare.
+  destruct (z1 ?= z2)%Z; simpl; tauto.
+Qed.
+
 
 Lemma if_false_is_and (b : Datatypes.bool) A : (if b then A else False) <-> (b = true /\ A).
 Proof.
@@ -227,3 +263,103 @@ Proof.
   destruct b; reflexivity.
 Qed.
 
+Lemma ex_order :
+  forall A B (P : A -> B -> Prop),
+    (exists x y, P x y) <->
+    (exists y x, P x y).
+Proof. split; intros [x [y HPxy]]; eauto. Qed.
+
+Lemma ex_eq_simpl :
+  forall A x P,
+    (exists x' : A, x' = x /\ P x') <->
+    P x.
+Proof.
+  intros A x P.
+  split.
+  - intros [x' [Hx Hp]]. congruence.
+  - intros Hp. exists x. intuition.
+Qed.
+
+Lemma iff_comm :
+  forall A B,
+    (A <-> B) <-> (B <-> A).
+Proof. intuition. Qed.
+
+Lemma and_pair_eq (A B : Type) (a c : A) (b d : B) : (a, b) = (c, d) <-> (a = c) /\ (b = d).
+Proof.
+  intuition. now inversion H. now inversion H.
+  congruence.
+Qed.
+
+Lemma ex_2 :
+  forall P Q,
+    (exists x : tez.mutez, (exists y : tez.mutez, P x y) /\ Q x) <->
+    (exists x y : tez.mutez, P x y /\ Q x).
+Proof. intuition; destruct H; destruct H; destruct H; eauto. Qed.
+
+Lemma underex_and_comm :
+  forall (A : Set) (P Q : A -> Prop),
+    (exists (x : A), P x /\ Q x) <->
+    (exists (x : A), Q x /\ P x).
+Proof.
+  intros A P Q. apply forall_ex. intuition.
+Qed.
+
+Lemma forall_ex2 {A : Set} {B : Set} {phi : A -> B -> Prop} {psi : A -> B -> Prop} :
+  (forall x y, phi x y <-> psi x y) -> (exists x y, phi x y) <-> (exists x y, psi x y).
+Proof. intros H. auto using forall_ex. Qed.
+
+Lemma underex2_and_comm :
+  forall (A B : Set) (P Q : A -> B -> Prop),
+    (exists (x : A) (y : B), P x y /\ Q x y) <->
+    (exists (x : A) (y : B), Q x y /\ P x y ).
+Proof. intros A B P Q. apply forall_ex2. intuition. Qed.
+
+Lemma underex2_and_assoc :
+  forall (A B : Set) (P Q R : A -> B -> Prop),
+    (exists (x : A) (y : B), (P x y /\ Q x y) /\ R x y) <->
+    (exists (x : A) (y : B), P x y /\ Q x y /\ R x y ).
+Proof.
+  intros A B P Q R.
+  apply forall_ex2. intros. apply and_assoc.
+Qed.
+
+Lemma ex2_and_comm {A : Set} {B : Set} {P : Prop} {Q : A -> B -> Prop} :
+  P /\ (exists x y, Q x y) <-> (exists x y, P /\ Q x y).
+Proof.
+  split.
+  intros [Hp [x [y Hq]]]. eauto.
+  intros [x [y [Hp Hq]]]. eauto.
+Qed.
+
+Lemma underex_and_assoc :
+  forall (A : Set) (P Q R : A -> Prop),
+    (exists (x : A), (P x /\ Q x) /\ R x) <->
+    (exists (x : A), P x /\ Q x /\ R x).
+Proof.
+  intros A P Q R.
+  apply forall_ex. intros. apply and_assoc.
+Qed.
+
+Lemma fold_right_psi_simpl :
+  forall (A B : Type) (psi : A -> Prop) (xs : Datatypes.list B)
+         (f  : (A -> Prop) -> B -> A -> Prop)
+         (f' : B -> A -> A)
+         (H : forall x st psi, f psi x st = psi (f' x st)),
+  forall st0,
+    List.fold_right (fun x psi st => f psi x st) psi xs st0 =
+    psi (List.fold_right f' st0 (List.rev xs)).
+Proof.
+  intros A B psi xs f f' H.
+  induction xs.
+  - now simpl.
+  - intro st0.
+    simpl.
+    rewrite H.
+    rewrite IHxs.
+    now rewrite List.fold_right_app.
+Qed.
+
+Lemma eq_iff_refl :
+  forall P Q, P = Q -> P <-> Q.
+Proof. intros. rewrite H. apply iff_refl. Qed.
